James C - started chapter 14

isabelle/Chapter14_1_Language.thy
@@ -1,201 +1,92 @@
 theory Chapter14_1_Language
-imports AssocList DeBruijn
+imports DeBruijnEnvironment
 begin
 
 datatype type = 
-  Nat 
-| Arr type type 
-| Unit 
-| Prod type type 
-| Void 
+  Nat
+| Arrow type type
+| Unit
+| Prod type type
+| Void
 | Sum type type
-| TyVar nat
-
-primrec is_type :: "nat => type => bool"
-where "is_type n Unit = True"
-    | "is_type n Nat = True"
-    | "is_type n (Sum t1 t2) = (is_type n t1 & is_type n t2)"
-    | "is_type n (Prod t1 t2) = (is_type n t1 & is_type n t2)"
-    | "is_type n (Arr t1 t2) = (is_type n t1 & is_type n t2)"
-    | "is_type n Void = True"
-    | "is_type n (TyVar x) = (x < n)"
-
-primrec occurs :: "nat => type => bool"
-where "occurs n Unit = False"
-    | "occurs n Nat = False"
-    | "occurs n (Sum t1 t2) = (occurs n t1 | occurs n t2)"
-    | "occurs n (Prod t1 t2) = (occurs n t1 | occurs n t2)"
-    | "occurs n (Arr t1 t2) = (occurs n t1 | occurs n t2)"
-    | "occurs n Void = False"
-    | "occurs n (TyVar x) = (x = n)"
-
-primrec is_positive :: "nat => type => bool"
-where "is_positive n Unit = True"
-    | "is_positive n Nat = True"
-    | "is_positive n (Sum t1 t2) = (is_positive n t1 & is_positive n t2)"
-    | "is_positive n (Prod t1 t2) = (is_positive n t1 & is_positive n t2)"
-    | "is_positive n (Arr t1 t2) = (~ occurs n t1 & is_positive n t2)"
-    | "is_positive n Void = True"
-    | "is_positive n (TyVar x) = True"
-
-primrec ty_subst :: "type => type => type"
-where "ty_subst t Unit = Unit"
-    | "ty_subst t Nat = Nat"
-    | "ty_subst t (Sum t1 t2) = Sum (ty_subst t t1) (ty_subst t t2)"
-    | "ty_subst t (Prod t1 t2) = Prod (ty_subst t t1) (ty_subst t t2)"
-    | "ty_subst t (Arr t1 t2) = Arr (ty_subst t t1) (ty_subst t t2)"
-    | "ty_subst t Void = Void"
-    | "ty_subst t (TyVar x) = (case x of 0 => t | Suc x' => TyVar x')"
-
-datatype patn =
-  PTriv
-| PPair
-| PInL
-| PInR
-| PZero
-| PSucc
-
-primrec vars_count :: "patn => nat"
-where "vars_count PTriv = 0"
-    | "vars_count PPair = 2"
-    | "vars_count PInL = 1"
-    | "vars_count PInR = 1"
-    | "vars_count PZero = 0"
-    | "vars_count PSucc = 1"
 
 datatype expr = 
-  Var nat 
+  Var var
 | Zero
-| Succ expr
+| Suc expr
+| Rec expr expr expr
 | Lam type expr
-| Ap expr expr
-| Fix type expr
+| Appl expr expr
 | Triv
 | Pair expr expr
 | ProjL expr
 | ProjR expr
 | Abort type expr
+| Case expr expr expr
 | InL type type expr
 | InR type type expr
-| Case expr type "rule list"
-| Map type expr expr
-and rule = Rule patn expr
 
-primrec free_vars :: "expr => nat set"
-    and free_vars_rules :: "rule list => nat set"
-    and free_vars_rule :: "rule => nat set"
-where "free_vars (Var v) = {v}"
-    | "free_vars Zero = {}"
-    | "free_vars (Succ e) = free_vars e"
-    | "free_vars (Lam t b) = redr_set (free_vars b)"
-    | "free_vars (Ap e1 e2) = free_vars e1 Un free_vars e2"
-    | "free_vars (Fix t b) = redr_set (free_vars b)"
-    | "free_vars Triv = {}"
-    | "free_vars (Pair e1 e2) = free_vars e1 Un free_vars e2"
-    | "free_vars (ProjL e) = free_vars e"
-    | "free_vars (ProjR e) = free_vars e"
-    | "free_vars (Abort t e) = free_vars e"
-    | "free_vars (InL t t' e) = free_vars e"
-    | "free_vars (InR t t' e) = free_vars e"
-    | "free_vars (Case e t rs) = free_vars e Un free_vars_rules rs"
-    | "free_vars (Map t e e') = redr_set (free_vars e) Un free_vars e'"
-    | "free_vars_rules Nil = {}"
-    | "free_vars_rules (r # rs) = free_vars_rule r Un free_vars_rules rs"    
-    | "free_vars_rule (Rule p e) = redr_set_by (vars_count p) (free_vars e)"
+primrec insert :: "var => expr => expr"
+where "insert n (Var v) = Var (incr n v)"
+    | "insert n Zero = Zero"
+    | "insert n (Suc e) = Suc (insert n e)"
+    | "insert n (Rec et e0 es) = Rec (insert n et) (insert n e0) (insert (next (next n)) es)"
+    | "insert n (Lam t e) = Lam t (insert (next n) e)"
+    | "insert n (Appl e1 e2) = Appl (insert n e1) (insert n e2)"
+    | "insert n Triv = Triv"
+    | "insert n (Pair e1 e2) = Pair (insert n e1) (insert n e2)"
+    | "insert n (ProjL e) = ProjL (insert n e)"
+    | "insert n (ProjR e) = ProjR (insert n e)"
+    | "insert n (Abort t e) = Abort t (insert n e)"
+    | "insert n (Case et el er) = Case (insert n et) (insert (next n) el) (insert (next n) er)"
+    | "insert n (InL t1 t2 e) = InL t1 t2 (insert n e)"
+    | "insert n (InR t1 t2 e) = InR t1 t2 (insert n e)"
 
-primrec incr_from :: "nat => expr => expr"
-    and incr_from_rules :: "nat => rule list => rule list"
-    and incr_from_rule :: "nat => rule => rule"
-where "incr_from n (Var v) = Var (incr n v)"
-    | "incr_from n Zero = Zero"
-    | "incr_from n (Succ e) = Succ (incr_from n e)"
-    | "incr_from n (Lam t b) = Lam t (incr_from (Suc n) b)"
-    | "incr_from n (Ap e1 e2) = Ap (incr_from n e1) (incr_from n e2)"
-    | "incr_from n (Fix t b) = Fix t (incr_from (Suc n) b)"
-    | "incr_from n Triv = Triv"
-    | "incr_from n (Pair e1 e2) = Pair (incr_from n e1) (incr_from n e2)"
-    | "incr_from n (ProjL e) = ProjL (incr_from n e)"
-    | "incr_from n (ProjR e) = ProjR (incr_from n e)"
-    | "incr_from n (Abort t e) = Abort t (incr_from n e)"
-    | "incr_from n (InL t t' e) = InL t t' (incr_from n e)"
-    | "incr_from n (InR t t' e) = InR t t' (incr_from n e)"
-    | "incr_from n (Case e t rs) = Case (incr_from n e) t (incr_from_rules n rs)"
-    | "incr_from n (Map t e e') = Map t (incr_from (Suc n) e) (incr_from n e')"
-    | "incr_from_rules n Nil = Nil"
-    | "incr_from_rules n (r # rs) = incr_from_rule n r # incr_from_rules n rs"    
-    | "incr_from_rule n (Rule p e) = Rule p (incr_from (n + vars_count p) e)"
+primrec remove :: "var => expr => expr"
+where "remove n (Var v) = Var (subr n v)"
+    | "remove n Zero = Zero"
+    | "remove n (Suc e) = Suc (remove n e)"
+    | "remove n (Rec et e0 es) = Rec (remove n et) (remove n e0) (remove (next (next n)) es)"
+    | "remove n (Lam t e) = Lam t (remove (next n) e)"
+    | "remove n (Appl e1 e2) = Appl (remove n e1) (remove n e2)"
+    | "remove n Triv = Triv"
+    | "remove n (Pair e1 e2) = Pair (remove n e1) (remove n e2)"
+    | "remove n (ProjL e) = ProjL (remove n e)"
+    | "remove n (ProjR e) = ProjR (remove n e)"
+    | "remove n (Abort t e) = Abort t (remove n e)"
+    | "remove n (Case et el er) = Case (remove n et) (remove (next n) el) (remove (next n) er)"
+    | "remove n (InL t1 t2 e) = InL t1 t2 (remove n e)"
+    | "remove n (InR t1 t2 e) = InR t1 t2 (remove n e)"
 
-lemma [simp]: "rs ~= [] ==> incr_from_rules n rs ~= []"
-by (cases rs, simp_all)
+primrec subst' :: "var => expr => expr => expr"
+where "subst' n e' (Var v) = (if v = n then e' else Var v)"
+    | "subst' n e' Zero = Zero"
+    | "subst' n e' (Suc e) = Suc (subst' n e' e)"
+    | "subst' n e' (Rec et e0 es) = 
+                      Rec (subst' n e' et) 
+                          (subst' n e' e0) 
+                          (subst' (next (next n)) (insert first (insert first e')) es)"
+    | "subst' n e' (Lam t e) = Lam t (subst' (next n) (insert first e') e)"
+    | "subst' n e' (Appl e1 e2) = Appl (subst' n e' e1) (subst' n e' e2)"
+    | "subst' n e' Triv = Triv"
+    | "subst' n e' (Pair e1 e2) = Pair (subst' n e' e1) (subst' n e' e2)"
+    | "subst' n e' (ProjL e) = ProjL (subst' n e' e)"
+    | "subst' n e' (ProjR e) = ProjR (subst' n e' e)"
+    | "subst' n e' (Abort t e) = Abort t (subst' n e' e)"
+    | "subst' n e' (Case et el er) = 
+                      Case (subst' n e' et) 
+                           (subst' (next n) (insert first e') el) 
+                           (subst' (next n) (insert first e') er)"
+    | "subst' n e' (InL t1 t2 e) = InL t1 t2 (subst' n e' e)"
+    | "subst' n e' (InR t1 t2 e) = InR t1 t2 (subst' n e' e)"
 
-lemma [simp]: "free_vars (incr_from n e) = incr n ` free_vars e"
-  and [simp]: "free_vars_rules (incr_from_rules k rs) = incr k ` free_vars_rules rs"
-  and [simp]: "free_vars_rule (incr_from_rule m r) = incr m ` free_vars_rule r"
-by (induction e and rs and r arbitrary: n and k and m, auto)
+definition subst :: "expr => expr => expr"
+where "subst e' e = remove first (subst' first (insert first e') e)"
 
-primrec incr_by :: "nat => expr => expr"
-where "incr_by 0 e = e"
-    | "incr_by (Suc n) e = incr_from 0 (incr_by n e)"
+lemma [simp]: "remove n (insert n e) = e"
+by (induction e arbitrary: n, simp_all)
 
-lemma [simp]:  "redr_set_by n (free_vars (incr_by n e)) = free_vars e" 
-by (induction n, simp_all) 
-
-primrec sub_from :: "nat => expr => expr"
-    and sub_from_rules :: "nat => rule list => rule list"
-    and sub_from_rule :: "nat => rule => rule"
-where "sub_from n (Var v) = Var (if v < n then v else if v = n then undefined else v - 1)"
-    | "sub_from n Zero = Zero"
-    | "sub_from n (Succ e) = Succ (sub_from n e)"
-    | "sub_from n (Lam t b) = Lam t (sub_from (Suc n) b)"
-    | "sub_from n (Ap e1 e2) = Ap (sub_from n e1) (sub_from n e2)"
-    | "sub_from n (Fix t b) = Fix t (sub_from (Suc n) b)"
-    | "sub_from n Triv = Triv"
-    | "sub_from n (Pair e1 e2) = Pair (sub_from n e1) (sub_from n e2)"
-    | "sub_from n (ProjL e) = ProjL (sub_from n e)"
-    | "sub_from n (ProjR e) = ProjR (sub_from n e)"
-    | "sub_from n (Abort t e) = Abort t (sub_from n e)"
-    | "sub_from n (InL t t' e) = InL t t' (sub_from n e)"
-    | "sub_from n (InR t t' e) = InR t t' (sub_from n e)"
-    | "sub_from n (Case e t rs) = Case (sub_from n e) t (sub_from_rules n rs)"
-    | "sub_from n (Map t e e') = Map t (sub_from (Suc n) e) (sub_from n e')"
-    | "sub_from_rules n Nil = Nil"
-    | "sub_from_rules n (r # rs) = sub_from_rule n r # sub_from_rules n rs"    
-    | "sub_from_rule n (Rule p e) = Rule p (sub_from (n + vars_count p) e)"
-
-lemma [simp]: "rs ~= [] ==> sub_from_rules n rs ~= []"
-by (cases rs, simp_all)
-
-primrec subst :: "expr => expr => nat => expr"
-    and subst_rules :: "rule list => expr => nat => rule list"
-    and subst_rule :: "rule => expr => nat => rule"
-where "subst (Var v) e x = (if v = x then e else Var v)"
-    | "subst Zero e x = Zero"
-    | "subst (Succ n) e x = Succ (subst n e x)"
-    | "subst (Lam t b) e x = Lam t (subst b (incr_from 0 e) (Suc x))"
-    | "subst (Ap e1 e2) e x = Ap (subst e1 e x) (subst e2 e x)"
-    | "subst (Fix t b) e x = Fix t (subst b (incr_from 0 e) (Suc x))"
-    | "subst Triv e x = Triv"
-    | "subst (Pair e1 e2) e x = Pair (subst e1 e x) (subst e2 e x)"
-    | "subst (ProjL n) e x = ProjL (subst n e x)"
-    | "subst (ProjR n) e x = ProjR (subst n e x)"
-    | "subst (Abort t n) e x = Abort t (subst n e x)"
-    | "subst (InL t t' n) e x = InL t t' (subst n e x)"
-    | "subst (InR t t' n) e x = InR t t' (subst n e x)"
-    | "subst (Case ec t rs) e x = Case (subst ec e x) t (subst_rules rs e x)"
-    | "subst (Map t e1 e2) e x = Map t (subst e1 (incr_from 0 e) (Suc x)) (subst e2 e x)"
-    | "subst_rules Nil e x = Nil"
-    | "subst_rules (r # rs) e x = subst_rule r e x # subst_rules rs e x"
-    | "subst_rule (Rule p b) e x = Rule p (subst b (incr_by (vars_count p) e) (x + vars_count p))"
-
-lemma [simp]: "rs ~= [] ==> subst_rules rs e x ~= []"
-by (cases rs, simp_all)
-
-definition safe_subst :: "expr => expr => expr"
-where "safe_subst e e' = sub_from 0 (subst e (incr_from 0 e') 0)"
-
-lemma [simp]: "free_vars (subst e e' x) = (if x : free_vars e then free_vars e - {x} Un free_vars e' else free_vars e)"
-  and [simp]: "free_vars_rules (subst_rules rs e'' y) = (if y : free_vars_rules rs then free_vars_rules rs - {y} Un free_vars e'' else free_vars_rules rs)"
-  and [simp]: "free_vars_rule (subst_rule r e''' z) = (if z : free_vars_rule r then free_vars_rule r - {z} Un free_vars e''' else free_vars_rule r)"
-by (induction e and rs and r arbitrary: e' x and e'' y and e''' z, auto)
+lemma [simp]: "canswap m n ==> insert m (insert n e) = insert (next n) (insert m e)"
+by (induction e arbitrary: n m, simp_all)
 
 end
