isabelle/Chapter14_3_Evaluation.thy
@@ -1,0 +1,145 @@
+theory Chapter14_3_Evaluation
+imports Chapter14_2_Typechecking
+begin
+
+primrec is_val :: "expr => bool"
+where "is_val (Var v) = False"
+    | "is_val Zero = True"
+    | "is_val (Suc e) = is_val e"
+    | "is_val (Rec et e0 es) = False"
+    | "is_val (Lam t e) = True"
+    | "is_val (Appl e1 e2) = False"
+    | "is_val Triv = True"
+    | "is_val (Pair e1 e2) = (is_val e1 & is_val e2)"
+    | "is_val (ProjL e) = False"
+    | "is_val (ProjR e) = False"
+    | "is_val (Abort t e) = False"
+    | "is_val (Case et el er) = False"
+    | "is_val (InL t1 t2 e) = is_val e"
+    | "is_val (InR t1 t2 e) = is_val e"
+
+inductive eval :: "expr => expr => bool"
+where eval_suc [simp]: "eval e e' ==> eval (Suc e) (Suc e')"
+    | eval_rec_1 [simp]: "eval et et' ==> eval (Rec et e0 es) (Rec et e0 es)"
+    | eval_rec_2 [simp]: "eval (Rec Zero e0 es) e0"
+    | eval_rec_3 [simp]: "is_val et ==> 
+            eval (Rec (Suc et) e0 es) (subst (Rec et e0 es) (subst et es))"
+    | eval_appl_1 [simp]: "eval e1 e1' ==> eval (Appl e1 e2) (Appl e1' e2)"
+    | eval_appl_2 [simp]: "is_val e1 ==> eval e2 e2' ==> eval (Appl e1 e2) (Appl e1 e2')"
+    | eval_appl_3 [simp]: "is_val e2 ==> eval (Appl (Lam t2 e1) e2) (subst e2 e1)"
+    | eval_pair_1 [simp]: "eval e1 e1' ==> eval (Pair e1 e2) (Pair e1' e2)"
+    | eval_pair_2 [simp]: "is_val e1 ==> eval e2 e2' ==> eval (Pair e1 e2) (Pair e1 e2')"
+    | eval_projl_1 [simp]: "eval e e' ==> eval (ProjL e) (ProjL e')"
+    | eval_projl_2 [simp]: "eval (ProjL (Pair e1 e2)) e1"
+    | eval_projr_1 [simp]: "eval e e' ==> eval (ProjR e) (ProjR e')"
+    | eval_projr_2 [simp]: "eval (ProjR (Pair e1 e2)) e2"
+    | eval_abort [simp]: "eval e e' ==> eval (Abort t e) (Abort t e')"
+    | eval_case_1 [simp]: "eval et et' ==> eval (Case et el er) (Case et el er)"
+    | eval_case_2 [simp]: "is_val e ==> eval (Case (InL t1 t2 e) el er) (subst e el)"
+    | eval_case_3 [simp]: "is_val e ==> eval (Case (InR t1 t2 e) el er) (subst e er)"
+    | eval_inl [simp]: "eval e e' ==> eval (InL t1 t2 e) (InL t1 t2 e')"
+    | eval_inr [simp]: "eval e e' ==> eval (InR t1 t2 e) (InR t1 t2 e')"
+
+lemma canonical_nat: "is_val e ==> typecheck gam e Nat ==> 
+          e = Zero | (EX e'. e = Suc e' & typecheck gam e' Nat)"
+by (induction e, auto)
+
+lemma canonical_nat_no_vars: "is_val e ==> typecheck gam e Nat ==> typecheck gam' e Nat"
+by (induction e, auto) 
+
+lemma canonical_arrow: "is_val e ==> typecheck gam e (Arrow t1 t2) ==> 
+              EX e'. e = Lam t1 e' & typecheck (extend gam t1) e' t2"
+by (induction e, auto)
+
+lemma canonical_triv: "is_val e ==> typecheck gam e Unit ==> e = Triv"
+by (induction e, auto)
+
+lemma canonical_pair: "is_val e ==> typecheck gam e (Prod t1 t2) ==> 
+              EX e1 e2. e = Pair e1 e2 & typecheck gam e1 t1 & typecheck gam e2 t2"
+by (induction e, auto)
+
+lemma canonical_void: "is_val e ==> typecheck gam e Void ==> False"
+by (induction e, auto)
+
+lemma canonical_sum: "is_val e ==> typecheck gam e (Sum t1 t2) ==> 
+          (EX e'. e = InL t1 t2 e' & typecheck gam e' t1) | 
+          (EX e'. e = InR t1 t2 e' & typecheck gam e' t2)"
+by (induction e, auto)
+
+theorem preservation: "eval e e' ==> typecheck gam e t ==> typecheck gam e' t"
+proof (induction e e' arbitrary: t rule: eval.induct)
+case eval_suc 
+  thus ?case by fastforce
+next case eval_rec_1 
+  thus ?case by fastforce
+next case eval_rec_2 
+  thus ?case by fastforce
+next case (eval_rec_3 et e0 es)
+  from eval_rec_3 canonical_nat_no_vars have "typecheck (extend gam t) (subst et es) t" by auto
+  with eval_rec_3 show ?case by fastforce
+next case eval_appl_1 
+  thus ?case by fastforce
+next case eval_appl_2 
+  thus ?case by fastforce
+next case eval_appl_3 
+  thus ?case by fastforce
+next case eval_pair_1 
+  thus ?case by fastforce
+next case eval_pair_2 
+  thus ?case by fastforce
+next case eval_projl_1 
+  thus ?case by fastforce
+next case eval_projl_2 
+  thus ?case by fastforce
+next case eval_projr_1 
+  thus ?case by fastforce
+next case eval_projr_2 
+  thus ?case by fastforce
+next case eval_abort
+  thus ?case by fastforce
+next case eval_case_1 
+  thus ?case by fastforce
+next case eval_case_2 
+  thus ?case by fastforce
+next case eval_case_3 
+  thus ?case by fastforce
+next case eval_inl
+  thus ?case by fastforce
+next case eval_inr
+  thus ?case by fastforce
+qed
+
+theorem progress: "typecheck gam e t ==> gam = empty_env ==> is_val e | (EX e'. eval e e')"
+proof (induction gam e t rule: typecheck.induct)
+case tc_var
+  thus ?case by simp
+next case tc_zero
+  thus ?case by simp
+next case tc_suc
+  thus ?case by (metis eval_suc is_val.simps(3))
+next case tc_rec
+  thus ?case by (metis eval_rec_1 eval_rec_2 eval_rec_3 is_val.simps(3) canonical_nat)
+next case tc_lam
+  thus ?case by simp
+next case tc_appl
+  thus ?case by (metis eval_appl_1 eval_appl_2 eval_appl_3 canonical_arrow)
+next case tc_triv
+  thus ?case by simp
+next case tc_pair
+  thus ?case by (metis eval_pair_1 eval_pair_2 is_val.simps(8))
+next case tc_projl
+  thus ?case by (metis eval_projl_1 eval_projl_2 canonical_pair)
+next case tc_projr
+  thus ?case by (metis eval_projr_1 eval_projr_2 canonical_pair)
+next case tc_abort
+  thus ?case by (metis eval_abort canonical_void)
+next case tc_case
+  thus ?case 
+  by (metis eval_case_1 eval_case_2 eval_case_3 is_val.simps(13) is_val.simps(14) canonical_sum)
+next case tc_inl
+  thus ?case by (metis eval_inl is_val.simps(13))
+next case tc_inr
+  thus ?case by (metis eval_inr is_val.simps(14))
+qed
+
+end
